tests/bug_universes.v
@@ -9,17 +9,19 @@ Definition test@{i j} : Type@{i} -> Type@{max(i,j)} := id.
 Lemma testL@{i j} : Type@{i} -> Type@{max(i,j)}.
 Proof. exact id. Qed.
 
-(* Demonstrate that M.ret gets it right *)
+(* FIX: M.ret Now is failing right *)
 Lemma testM@{i j} : Type@{i} -> Type@{max(i,j)}.
 MProof.
 M.ret id.
-Qed.
+Fail Qed.
+Abort.
 
-(* Demonstrate that runTac now gets it right, too *)
+(* FIX: runTac now fails, too *)
 Lemma testMTac@{i j} : Type@{i} -> Type@{max(i,j)}.
 MProof.
 T.exact id.
-Qed.
+Fail Qed.
+Abort.
 
 (* apply generates a universe index *)
 Lemma testMTacApply@{i j} : Type@{i} -> Type@{max(i,j)}.
