tests/test_escaped_var.v
@@ -6,11 +6,13 @@ Import M.notations.
 Definition anat : nat.
 MProof.
   _ <- M.evar nat; M.ret 0.
-MQed.
+  Unshelve.
+MQed. (* Shouldn't it be better to not have to Unshelve? *)
 
 Definition escaped_evar : nat.
 MProof.
 x <- M.evar nat; M.ret x.
+Unshelve.
 Fail MQed. (* OK, the goal was not solved *)
 M.ret 0.
 Fail MQed. (* OK, no need for MQed, no goal is open (although we might want to have MQed work here) *)
